Improve Signal specification

fstar/Spec.Signal.Core.fst
@@ -11,94 +11,6 @@ open Spec.Signal.Messages
 #set-options "--z3rlimit 50 --fuel 0 --ifuel 0"
 
 
-let verify_sig (identity_key:pubkey) (signed_pub_key: pubkey) (signature:lbytes 64) : Tot bool =
-  verify identity_key signed_pub_key signature
-
-let sign (priv_key:privkey) (pub_key:pubkey) : Tot (lbytes 64) =
-  sign priv_key pub_key
-
-
-let ratchet
-    (root_key:key)                   (* $rk_j$    *)
-    (our_ephemeral_priv_key:privkey) (* $x_j$     *)
-    (their_ephemeral_pub_key:pubkey) (* $g^{y_j}$ *)
-    : Tot (key & key) =              (* output: $rk_{j+1}, ck_{j+1,0}$ *)
-
-  let shared_secret =
-    dh our_ephemeral_priv_key their_ephemeral_pub_key in
-  let keys = hkdf2 shared_secret root_key label_WhisperRatchet in
-  let root_key' = sub keys 0 32 in
-  let chain_key = sub keys 32 32 in
-  (root_key', chain_key)
-
-
-let initiate'
-    (our_identity_priv_key: privkey) (* $i$   *)
-    (our_onetime_priv_key: privkey)  (* $e$   *)
-    (their_identity_pub_key: pubkey) (* $g^r$ *)
-    (their_signed_pub_key: pubkey)   (* $g^s$ *)
-    (their_onetime_pub_key: option pubkey)  (* $g^o$, optional *)
-    : Tot (lbytes 32) =                    (* output: $rk_0$ *)
-
-  let dh1 = dh our_identity_priv_key their_signed_pub_key in
-  let dh2 = dh our_onetime_priv_key their_identity_pub_key in
-  let dh3 = dh our_onetime_priv_key their_signed_pub_key in
-  let shared_secret =
-    match their_onetime_pub_key with
-    | None -> ff @| dh1 @| dh2 @| dh3
-    | Some their_onetime_pub_key ->
-	   let dh4 = dh our_onetime_priv_key their_onetime_pub_key in
-	   ff @| dh1 @| dh2 @| dh3 @| dh4 in
-  let res = hkdf1 shared_secret zz label_WhisperText in
-  res
-
-
-let initiate
-    (our_identity_priv_key: privkey) (* $i$   *)
-    (base_priv_key: privkey)
-    (our_onetime_priv_key: privkey)  (* $e$   *)
-    (their_identity_pub_key: pubkey) (* $g^r$ *)
-    (their_signed_pub_key: pubkey)   (* $g^s$ *)
-    (their_onetime_pub_key: option pubkey)  (* $g^o$, optional *)
-    : Tot (key & key) =
-  let root_key0 = initiate'
-    our_identity_priv_key
-    base_priv_key
-    their_identity_pub_key
-    their_signed_pub_key
-    their_onetime_pub_key
-  in
-  ratchet root_key0 our_onetime_priv_key their_signed_pub_key
-
-
-let respond
-  (our_identity_priv_key: privkey) (* $r$ *)
-  (our_signed_priv_key: privkey)   (* $s$ *)
-  (our_onetime_priv_key: option privkey)  (* $o$, optional *)
-  (their_identity_pub_key: pubkey) (* $g^i$ *)
-  (their_onetime_pub_key: pubkey)  (* $g^e$ *)
-  : Tot (root_key:key) =                    (* output: $rk_0$ *)
-  let dh1 = dh our_signed_priv_key their_identity_pub_key in
-  let dh2 = dh our_identity_priv_key their_onetime_pub_key in
-  let dh3 = dh our_signed_priv_key their_onetime_pub_key in
-  let shared_secret =
-    match our_onetime_priv_key with
-    | None -> ff @| dh1 @| dh2 @| dh3
-    | Some our_onetime_priv_key ->
-	let dh4 = dh our_onetime_priv_key their_onetime_pub_key in
-	ff @| dh1 @| dh2 @| dh3 @| dh4
-  in
-  hkdf1 shared_secret zz label_WhisperText
-
-
-let fill_message_keys
-    (chain_key:privkey)
-    : Tot (privkey & privkey) =
-  let msg_key = hmac chain_key one in
-  let chain_key' = hmac chain_key two in
-  msg_key, chain_key'
-
-
 let size_encrypt_max_length
   (plen:size_nat{plen + 16 <= max_size_t /\ cipherlen plen + 140 <= max_size_t})
   : size_nat =
@@ -112,57 +24,143 @@ let encrypt_get_length
     1 + (serialize_whisper_message_get_length prev_counter counter (cipherlen plen)) + 8
 
 
-let encrypt
-    (our_identity_pub_key:pubkey)    (* $g^i$ or $g^r$ *)
-    (their_identity_pub_key:pubkey)  (* $g^r$ or $g^i$ *)
-    (msg_key:key)                    (* $ck_j$ *)
-    (our_ephemeral_pub_key:pubkey)   (* $g^{x}$ *)
-    (prev_counter:size_nat)          (* previous $k$ *)
-    (counter:size_nat)               (* current  $j$ *)
-    (plaintext:plain_bytes)	     (* message $m_j$ *)
-    : Tot (lbytes (encrypt_get_length prev_counter counter (length plaintext))) =
-    (* output: $c_j$, $t_j$, $ck_{j+1}$ *)
+
+val verify_sig: identity_key:pubkey -> signed_pub_key: pubkey -> signature:lbytes 64 -> Tot bool
+let verify_sig identity_key signed_pub_key signature =
+  verify identity_key signed_pub_key signature
+
+
+val sign: priv_key:privkey -> pub_key:pubkey -> Tot (lbytes 64)
+let sign priv_key pub_key = sign priv_key pub_key
+
+
+val ratchet:
+  root_key: key ->                   (* $rk_j$    *)
+  our_ephemeral_priv_key: privkey -> (* $x_j$     *)
+  their_ephemeral_pub_key: pubkey -> (* $g^{y_j}$ *)
+  Tot (key & key)              (* output: $rk_{j+1}, ck_{j+1,0}$ *)
+
+let ratchet rk sesk repk =
+  let ss = dh sesk repk in
+  let keys = hkdf2 ss rk label_WhisperRatchet in
+  let rk' = sub keys 0 32 in
+  let ck = sub keys 32 32 in
+  (rk', ck)
+
+
+val initiate':
+  our_identity_priv_key: privkey -> (* $i$   *)
+  our_onetime_priv_key: privkey ->  (* $e$   *)
+  their_identity_pub_key: pubkey -> (* $g^r$ *)
+  their_signed_pub_key: pubkey ->   (* $g^s$ *)
+  their_onetime_pub_key: option pubkey ->  (* $g^o$, optional *)
+  Tot (lbytes 32)                    (* output: $rk_0$ *)
+
+let initiate' iidsk iesk ridpk rspk orepk =
+  let dh1 = dh iidsk rspk in
+  let dh2 = dh iesk ridpk in
+  let dh3 = dh iesk rspk in
+  let ss =
+    match orepk with
+    | None -> ff @| dh1 @| dh2 @| dh3
+    | Some repk ->
+	   let dh4 = dh iesk repk in
+	   ff @| dh1 @| dh2 @| dh3 @| dh4 in
+  let res = hkdf1 ss zz label_WhisperText in
+  res
+
+
+val initiate:
+  our_identity_priv_key: privkey -> (* $i$   *)
+  base_priv_key: privkey ->
+  our_onetime_priv_key: privkey ->  (* $e$   *)
+  their_identity_pub_key: pubkey -> (* $g^r$ *)
+  their_signed_pub_key: pubkey ->   (* $g^s$ *)
+  their_onetime_pub_key: option pubkey ->  (* $g^o$, optional *)
+  Tot (key & key)
+
+let initiate iidsk bsk iesk ridpk rspk repk =
+  let rk0 = initiate' iidsk bsk ridpk rspk repk in
+  ratchet rk0 iesk rspk
+
+
+val respond:
+  our_identity_priv_key: privkey -> (* $r$ *)
+  our_signed_priv_key: privkey ->   (* $s$ *)
+  our_onetime_priv_key: option privkey ->  (* $o$, optional *)
+  their_identity_pub_key: pubkey -> (* $g^i$ *)
+  their_onetime_pub_key: pubkey ->  (* $g^e$ *)
+  Tot (root_key:key)                   (* output: $rk_0$ *)
+
+let respond ridsk rssk oresk sidpk iepk =
+  let dh1 = dh rssk sidpk in
+  let dh2 = dh ridsk iepk in
+  let dh3 = dh rssk iepk in
+  let ss =
+    match oresk with
+    | None -> ff @| dh1 @| dh2 @| dh3
+    | Some resk ->
+	   let dh4 = dh resk iepk in
+	   ff @| dh1 @| dh2 @| dh3 @| dh4 in
+  hkdf1 ss zz label_WhisperText
+
+
+val fill_message_keys: chain_key:privkey -> Tot (privkey & privkey)
+let fill_message_keys ck =
+  let msg_key = hmac ck one in
+  let chain_key' = hmac ck two in
+  msg_key, chain_key'
+
+
+val encrypt:
+  our_identity_pub_key:pubkey ->    (* $g^i$ or $g^r$ *)
+  their_identity_pub_key:pubkey ->  (* $g^r$ or $g^i$ *)
+  msg_key:key ->                    (* $ck_j$ *)
+  our_ephemeral_pub_key:pubkey ->   (* $g^{x}$ *)
+  prev_counter:size_nat ->          (* previous $k$ *)
+  counter:size_nat ->               (* current  $j$ *)
+  plaintext:plain_bytes ->	     (* message $m_j$ *)
+  Tot (lbytes (encrypt_get_length prev_counter counter (length plaintext)))
+  (* output: $c_j$, $t_j$, $ck_{j+1}$ *)
+
+let encrypt sidpk ridpk msg_key sepk pctr ctr plaintext =
   let keys = hkdf3 msg_key zz label_WhisperMessageKeys in
   let enc_key = sub keys 0 32 in
   let mac_key = sub keys 32 32 in
   let enc_iv  = sub keys 64 16 in
   let ciphertext = aes_enc enc_key enc_iv plaintext in
   (* FStarEncrypt returns here with (ciphertext & mac_key) *)
-  let whisper_msg = serialize_whisper_message our_ephemeral_pub_key
-		      prev_counter counter ciphertext in
+  let whisper_msg = serialize_whisper_message sepk pctr ctr ciphertext in
   (* BB: 2019/11/04 *)
   assume(length whisper_msg + size_mac_whisper_msg_extra_info +
     Spec.Hash.Definitions.block_length (Spec.Hash.Definitions.SHA2_256) < max_size_t);
-  let tag8 : lbytes 8 = mac_whisper_msg mac_key their_identity_pub_key our_identity_pub_key whisper_msg in
+  let tag8 : lbytes 8 = mac_whisper_msg mac_key ridpk sidpk whisper_msg in
   let c0 : lbytes 1 = create 1 (((u8 3) <<. (size 4)) |. (u8 3)) in
   let output = concat (concat c0 (to_lseq whisper_msg)) tag8 in
   output
 
 
-let decrypt
-    (our_identity_pub_key:pubkey)    // $g^i$ or $g^r$
-    (their_identity_pub_key:pubkey)  // $g^r$ or $g^i$
-    (remote_ephemeral_key:pubkey)
-    (msg_key:key)                  // $ck_j$
-    (prev_counter:size_nat)          // prev msg number $k$
-    (counter:size_nat)               // current msg number $j$
-    (ciphertext:cipher_bytes)	       // ciphertext $c_j$
-    (tag8:lbytes 8)                  // tag $t_j$
-    : Tot (option (plain_bytes)) =   // outputs: $m_j$, $ck_{j+1}$
+val decrypt:
+  our_identity_pub_key:pubkey ->    // $g^i$ or $g^r$
+  their_identity_pub_key:pubkey ->  // $g^r$ or $g^i$
+  remote_ephemeral_key:pubkey ->
+  msg_key:key ->                  // $ck_j$
+  prev_counter:size_nat ->          // prev msg number $k$
+  counter:size_nat ->               // current msg number $j$
+  ciphertext:cipher_bytes ->	       // ciphertext $c_j$
+  tag8:lbytes 8 ->                  // tag $t_j$
+  Tot (option (plain_bytes))  // outputs: $m_j$, $ck_{j+1}$
 
+let decrypt ridpk sidpk repk msg_key pctr ctr ciphertext tag8 =
   let len = length ciphertext in
   let ciphertext = to_lseq ciphertext in
   let keys = hkdf3 msg_key zz label_WhisperMessageKeys in
   let enc_key = sub keys 0 32 in
   let mac_key = sub keys 32 32 in
   let enc_iv  = sub keys 64 16 in
-  let whisper_message =
-    serialize_whisper_message remote_ephemeral_key prev_counter counter ciphertext
-  in
-  let exp_tag8 =
-    mac_whisper_msg mac_key our_identity_pub_key their_identity_pub_key whisper_message in
-  if not (equal_bytes tag8 exp_tag8) then
-    None
+  let whisper_message = serialize_whisper_message repk pctr ctr ciphertext in
+  let exp_tag8 = mac_whisper_msg mac_key ridpk sidpk whisper_message in
+  if not (equal_bytes tag8 exp_tag8) then None
   else
     let plain = aes_dec enc_key enc_iv ciphertext in
     match plain with
@@ -170,6 +168,7 @@ let decrypt
     | None -> None
 
 
-let generate_key_pair (e: Ghost.erased entropy) : Tot (privkey & pubkey) =
+val generate_key_pair: (e: Ghost.erased entropy) -> Tot (privkey & pubkey)
+let generate_key_pair e =
   let priv = random_bytes e 32 in
   (priv, priv_to_pub priv)
